\begin{equation}
  \begin{aligned}
    k_{i}                & = a_{i} \exp(-\frac{E_{i}}{R T_{R}})
    \\
    \frac{d}{dt}C_{A}(t) & = -k_1 C_{T}(t) C_{A}(t) + k_2 C_{D}(t) C_{E}(t) - k_3 C_{D}(t) C_{A}(t) + k_4 C_{M}(t) C_{E}(t) - k_5 C_{M}(t) C_{A}(t) + k_6 C_{G}(t) C_{E}(t)
    \\
    \frac{d}{dt}C_{T}(t) & = -k_1 C_{T}(t) C_{A}(t) + k_2 C_{D}(t) C_{E}(t)
    \\
    \frac{d}{dt}C_{D}(t) & = k_1 C_{T}(t) C_{A}(t) - k_2 C_{D}(t) C_{E}(t) - k_3 C_{D}(t) C_{A}(t) + k_4 C_{M}(t) C_{E}(t)
    \\
    \frac{d}{dt}C_{M}(t) & = k_3 C_{D}(t) C_{A}(t) - k_4 C_{M}(t) C_{E}(t) - k_5 C_{M}(t) C_{A}(t) + k_6 C_{G}(t) C_{E}(t)
    \\
    \frac{d}{dt}C_{G}(t) & = k_5 C_{M}(t) C_{A}(t) - k_6 C_{G}(t) C_{E}(t)
    \\
    \frac{d}{dt}C_{E}(t) & = k_1 C_{T}(t) C_{A}(t) - k_2 C_{D}(t) C_{E}(t) + k_3 C_{D}(t) C_{A}(t) - k_4 C_{M}(t) C_{E}(t) + k_5 C_{M}(t) C_{A}(t) - k_6 C_{G}(t) C_{E}(t)
  \end{aligned}
  \label{eq:biodiesel01_2_1}
\end{equation}
