\begin{equation}
  \begin{aligned}
    - r_{A}               & = kC_{A}(t)
    \\
    k                     & = k_{0} \exp(\frac{-E}{RT(t)})
    \\
    Q                     & = \frac{aF_{c}^{b+1}}{F_{c} + (\frac{aF_{c}^{b}}{2\rho_{c}c_{p}})}(T(t)-T_{c})
    \\
    \frac{d}{dt} C_{A}(t) & = \frac{F}{V}[C_{0} - C_{A}(t)] + r_{A}
    \\
    \frac{dT(t)}{dt}      & = \frac{F}{V} [T_{0}-T(t)] + \frac{h_{r}}{\rho C_{p}}r_{A} - \frac{Q}{\rho c_{p} V}
    \label{eq:CSTR_1storder02_1}
  \end{aligned}
\end{equation}
